src/Narcissus/Formats.v
@@ -7,4 +7,5 @@ Require Export
         Fiat.Narcissus.Formats.SumTypeOpt
         Fiat.Narcissus.Formats.IPChecksum
         Fiat.Narcissus.Formats.WordOpt
+        Fiat.Narcissus.Formats.FixFormat
         Fiat.Narcissus.Formats.NatOpt.
